WIP and attempt proof FTLR restrict

theories/ftlr/Restrict.v
@@ -38,140 +38,368 @@ Section fundamental.
     iApply (interp_weakening with "IH HIDC") ; eauto ; try solve_addr.
   Qed.
 
-  Definition reg_allows_IE (regs : Reg) (r : RegName) b e a :=
-    regs !! r = Some (WCap IE b e a) ∧
-    withinBounds b e a = true /\
-    withinBounds b e (a^+1)%a = true.
+  Definition reg_allows_read_IE (regs : Reg) (r : RegName) p b e a :=
+    regs !! r = Some (WCap p b e a)
+    /\ readAllowed p = true
+    ∧ withinBounds b e a = true
+    ∧ withinBounds b e (a^+1)%a = true.
 
   (* The necessary resources to close the region again,
      except for the points to predicate, which we will store separately *)
-  Definition region_open_resources (pc_a : Addr) (w1 w2 : Word) (a : Addr) : iProp Σ :=
-    (▷ interp w1 ∗ ▷ interp w2 ∗
-       ((▷ ∃ w, a ↦ₐ w ∗ interp w) ∗ (▷ ∃ w, (a^+1)%a ↦ₐ w ∗ interp w)
-        ={⊤ ∖ ↑logN.@pc_a ∖ ↑logN.@a ∖ ↑logN.@(a^+1)%a, ⊤ ∖ ↑logN.@pc_a}=∗ emp)
+  Definition region_open_resources (Pa Pa' : D) (pc_a : Addr) (w1 w2 : Word) (a : Addr) (f:bool) : iProp Σ :=
+    ((if f then ▷ Pa w1 else Pa w1) ∗ read_cond Pa interp ∗
+       (if f then ▷ Pa' w2 else Pa' w2) ∗ read_cond Pa' interp
+       (* Close the invariant for a *)
+       ∗ ((▷ ∃ w1, a ↦ₐ w1 ∗ Pa w1) ={⊤ ∖ ↑logN.@pc_a ∖ ↑logN.@a,⊤ ∖ ↑logN.@pc_a}=∗ emp)
+       (* Close the invariant for (a+1) *)
+       ∗ ((▷ ∃ w2, (a ^+ 1)%a ↦ₐ w2  ∗ Pa' w2) ={⊤ ∖ ↑logN.@pc_a ∖ ↑logN.@a ∖ ↑logN.@(a ^+ 1)%a,
+           ⊤ ∖ ↑logN.@pc_a ∖ ↑logN.@a}=∗ emp)
     )%I.
 
-  (* Description of what the resources are supposed to look like after
-     opening the region if we need to, but before closing the region up again *)
-  Definition allow_IE_res (r : RegName) (regs : Reg) pc_a p b e a :=
-    (⌜read_reg_inr regs r p b e a⌝ ∗
-      (if decide (reg_allows_IE regs r b e a ∧ a ≠ pc_a /\ (a^+1)%a ≠ pc_a)
-       then |={⊤ ∖ ↑logN.@pc_a,⊤ ∖ ↑logN.@pc_a ∖ ↑logN.@a ∖ ↑logN.@(a^+1)%a}=>
-              ∃ w1 w2, a ↦ₐ w1 ∗ (a^+1)%a ↦ₐ w2 ∗ region_open_resources pc_a w1 w2 a
-    else True))%I.
+  Definition allow_restrict_res
+    (regs : leibnizO Reg) (dst : RegName)
+    (pc_a : Addr) (p : Perm)
+    (b e a : Addr) (Pa Pa' : D)
+    :=
+    (⌜read_reg_inr regs dst p b e a⌝ ∗
+    if decide (reg_allows_read_IE regs dst p b e a ∧ a ≠ pc_a ∧ (a^+1)%a ≠ pc_a)
+    then |={⊤ ∖ ↑logN.@pc_a,⊤ ∖ ↑logN.@pc_a ∖ ↑logN.@a ∖ ↑logN.@(a^+1)%a}=>
+           ∃ w1 w2, a ↦ₐ w1
+                      ∗ (a^+1)%a ↦ₐ w2
+                      ∗ region_open_resources Pa Pa' pc_a w1 w2 a true
+                      ∗ ▷ interp w1
+                      ∗ ▷ interp w2
+     else True)%I.
 
-  Definition allow_IE_mem (r : RegName) (regs : Reg) pc_a pc_w (mem : Mem) p b e a :=
-    (⌜read_reg_inr regs r p b e a⌝ ∗
-      (if decide (reg_allows_IE regs r b e a ∧ a ≠ pc_a /\ (a^+1)%a ≠ pc_a)
-       then ∃ w1 w2,
-           ⌜mem = <[(a^+1)%a:=w2]> (<[a:=w1]> (<[pc_a:=pc_w]> ∅))⌝
-                                     ∗ region_open_resources pc_a w1 w2 a
-       else ⌜mem = (<[pc_a:=pc_w]> ∅)⌝))%I.
-
-  Lemma indirect_sentry_allowed_inv (b e a: Addr) :
-    (b ≤ a ∧ a < e)%Z →
-    (b ≤ (a^+1)%a ∧ (a^+1)%a < e)%Z →
-    ⊢ (interp (WCap IE b e a) →
-       ∃ w1 w2,
-         inv (logN .@ a) (a ↦ₐ w1) ∗ inv (logN .@ (a^+1)%a) ((a^+1)%a ↦ₐ w2))%I.
+  Lemma create_restrict_res:
+    ∀ (regs : leibnizO Reg) (dst : RegName)
+      (p_pc : Perm) (b_pc e_pc a_pc : Addr)
+      (p : Perm) (b e a : Addr),
+      read_reg_inr (<[PC:=WCap p_pc b_pc e_pc a_pc]> regs) dst p b e a
+      → (∀ (r : RegName) (w : Word),
+            ⌜r ≠ PC⌝ → ⌜r ≠ idc⌝ → ⌜regs !! r = Some w⌝ → (fixpoint interp1) w)
+        -∗ ∃ Pa Pa', allow_restrict_res (<[PC:=WCap p_pc b_pc e_pc a_pc]> regs) dst a_pc p b e a Pa Pa'.
   Proof.
-    iIntros ([Ha_b Ha_e] [Ha_b' Ha_e']) "#Hinterp".
-    rewrite /interp //= fixpoint_interp1_eq /=; cbn.
-    assert (withinBounds b e a) as Hwb. admit.
-    assert (withinBounds b e (a^+1)%a) as Hwb'. admit.
+    intros regs dst p_pc b_pc e_pc a_pc p b e a HVdst.
+    iIntros "Hreg". rewrite /allow_restrict_res.
+    iFrame "%".
+    case_decide as Hdec; [|iExists (λne _, True%I), (λne _, True%I);done].
+    destruct Hdec as (Hallows & Haeq &Ha'eq).
+    destruct Hallows as (Hrinr & Hra & Hwb & Hwb').
+
+    apply andb_prop in Hwb as [Hle Hge].
+    apply andb_prop in Hwb' as [Hle' Hge'].
+    assert (a <> a^+ 1)%a as Ha_a' by solve_addr.
+
+    (* We prove that dst could not have been the PC, since the PC can't be an IE-cap *)
+    assert (dst ≠ PC) as Hdst_pc.
+    { refine (addr_ne_reg_ne Hrinr _ Haeq); by rewrite lookup_insert. }
+    rewrite lookup_insert_ne in Hrinr; last by congruence.
+    destruct (decide (dst = idc)) as [? | Hdst_idc]; simplify_map_eq.
+    - (* dst = idc *)
+      admit. (* By IH, I know already know V(widc) ? *)
+    - (* dst ≠ idc *)
+      iDestruct ("Hreg" $! dst _ Hdst_pc Hdst_idc Hrinr) as "#Hvdst".
+
+      iDestruct (read_allowed_inv a with "Hvdst") as (Pa) "[Hinv_a [Hconds_a _] ]"; auto;
+        first (split; [by apply Z.leb_le | by apply Z.ltb_lt]).
+
+      iDestruct (read_allowed_inv (a^+1)%a with "Hvdst") as (Pa') "[Hinv_a' [Hconds_a' _] ]"; auto;
+        first (split; [by apply Z.leb_le | by apply Z.ltb_lt]).
+      iExists Pa, Pa'.
+
+      (* TODO is there a better way to open multiple invariant at once ? *)
+      iMod (inv_acc (⊤ ∖ ↑logN.@a_pc) with "Hinv_a") as "[Hrefa Hcls]";[solve_ndisj|].
+      iMod (inv_acc (⊤ ∖ ↑logN.@a_pc ∖ ↑logN.@a) with "Hinv_a'") as "[Hrefa' Hcls']";[solve_ndisj|].
+      iDestruct "Hrefa" as (w1) "[>Ha HPa]".
+      iDestruct "Hrefa'" as (w2) "[>Ha' HPa']".
+      iExists w1, w2.
+      iAssert (▷ interp w1)%I as "#Hw1".
+      { iNext. iApply "Hconds_a". iFrame. }
+      iAssert (▷ interp w2)%I as "#Hw2".
+      { iNext. iApply "Hconds_a'". iFrame. }
+      rewrite /interp_ref_inv /=. iFrame "∗ #". done.
   Admitted.
 
-  (* Lemma create_IE_res: *)
-  (*   ∀ (regs : leibnizO Reg) (p : Perm) (b e a : Addr) *)
-  (*     (r : RegName) (b0 e0 a0 : Addr), *)
-  (*     r <> idc (* TODO *) *)
-  (*     -> read_reg_inr (<[PC:=WCap p b e a]> regs) r IE b0 e0 a0 *)
-  (*     → (∀ (r' : RegName) v, ⌜r' ≠ PC⌝ → ⌜r' ≠ idc⌝ → ⌜regs !! r' = Some v⌝ → (fixpoint interp1) v) *)
-  (*         -∗ allow_IE_res r (<[PC:=WCap p b e a]> regs) a IE b0 e0 a0. *)
-  (* Proof. *)
-  (*   intros regs p b e a r b0 e0 a0 Hr_idc HVr. *)
-  (*   iIntros "#Hreg". *)
-  (*   iFrame "%". *)
-  (*   case_decide as Hallows. *)
-  (*   - destruct Hallows as ((Hrinr & Hwb & Hwb') & Haeq & Ha'eq). *)
-  (*     apply andb_prop in Hwb as [Hle Hge]. *)
-  (*     apply andb_prop in Hwb' as [Hle' Hge']. *)
-  (*     revert Hle Hge; rewrite !Z.leb_le Z.ltb_lt =>Hle Hge. *)
-  (*     revert Hle' Hge'; rewrite !Z.leb_le Z.ltb_lt =>Hle' Hge'. *)
-  (*     assert (r ≠ PC) as Hr_pc. *)
-  (*     { refine (addr_ne_reg_ne Hrinr _ Haeq); by rewrite lookup_insert. } *)
-  (*     (* assert (r ≠ idc) as Hr_idc. *) *)
-  (*     (* { refine (addr_ne_reg_ne Hrinr _ Haeq). rewrite lookup_insert. } *) *)
-  (*   rewrite lookup_insert_ne in Hrinr; last by congruence. *)
-  (*   iDestruct ("Hreg" $! r _ Hr_pc Hr_idc Hrinr) as "Hvsrc". *)
-  (*   iAssert (∃ w1 w2, inv (logN.@a0) (a0 ↦ₐ w1) *)
-  (*                       ∗ inv (logN.@(a0^+1)%a) ((a0^+1)%a ↦ₐ w2))%I *)
-  (*     as (w1 w2) "[#Hinva #Hinva']". *)
-  (*   { iDestruct (indirect_sentry_allowed_inv with "Hvsrc") as (w1 w2) "[Hw1 Hw2]" *)
-  (*     ; auto. } *)
-  (*   iExists w1, w2. *)
-  (*   iFrame "∗ #". *)
-  (*   iMod (inv_acc with "Hinva") as "[>Ha0 Hcls']";[solve_ndisj|]. *)
-  (*   iMod (inv_acc with "Hinva'") as "[>Ha0' Hcls'']";[admit|]. *)
-  (*   iFrame. *)
-  (*   rewrite /region_open_resources. *)
-  (*   done. *)
-  (*   - done. *)
-  (* Qed. *)
+  Definition allow_read_IE_mem
+    (mem : Mem) (regs : Reg) (dst : RegName)
+    (pc_a : Addr) (pc_w : Word)
+    (p : Perm) (b e a : Addr) (Pa Pa':D) (f:bool): iPropI Σ :=
+    (⌜read_reg_inr regs dst p b e a⌝ ∗
+       if decide (reg_allows_read_IE regs dst p b e a ∧ a ≠ pc_a ∧ (a^+1)%a ≠ pc_a)
+       then ∃ (w1 w2 : Word),
+           ⌜mem = <[(a^+1)%a := w2]> (<[a := w1]> ∅)⌝
+           ∗ (region_open_resources Pa Pa' pc_a w1 w2 a f)
+           ∗ (if f then ▷ interp w1 else interp w1)
+           ∗ (if f then ▷ interp w2 else interp w2)
+       else  ⌜mem = ∅⌝)%I.
+
+   (* TODO move *)
+   Lemma memMap_resource_3ne (a1 a2 a3 : Addr) (w1 w2 w3 : Word)  :
+    a1 ≠ a2 →
+    a1 ≠ a3 →
+    a2 ≠ a3 →
+    ([∗ map] a↦w ∈ <[a1:=w1]> (<[a2:=w2]> (<[a3:=w3]> ∅)),
+      a ↦ₐ w)%I
+      ⊣⊢ a1 ↦ₐ w1 ∗ a2 ↦ₐ w2 ∗ a3 ↦ₐ w3.
+  Proof.
+    intros.
+    rewrite big_sepM_delete; last by apply lookup_insert.
+  Admitted.
+
+  Lemma restrict_res_implies_mem_map:
+    ∀ (regs : leibnizO Reg) (dst : RegName)
+      (pc_a : Addr) (pc_w : Word)
+      (p : Perm) (b e a : Addr)
+      (Pa Pa' : D),
+      allow_restrict_res regs dst pc_a p b e a Pa Pa'
+      -∗ pc_a ↦ₐ pc_w
+      ={⊤ ∖ ↑logN.@pc_a,
+        if decide (reg_allows_read_IE regs dst p b e a ∧ a ≠ pc_a ∧ (a^+1)%a ≠ pc_a)
+        then ⊤ ∖ ↑logN.@pc_a ∖ ↑logN.@a ∖ ↑logN.@(a ^+ 1)%a
+        else ⊤ ∖ ↑logN.@pc_a}=∗
+        ∃ mem : Mem,
+          allow_read_IE_mem mem regs dst pc_a pc_w p b e a Pa Pa' true
+            ∗ ▷ (([∗ map] a0↦w ∈ mem, a0 ↦ₐ w) ∗ pc_a ↦ₐ pc_w).
+  Proof.
+    intros regs dst pc_a pc_w p b e a Pa Pa'.
+    iIntros "HRestrictRes Hpc_a".
+    iDestruct "HRestrictRes" as "[% HRestrictRes]".
+    case_decide as Hdec. destruct Hdec as (Hallows & Haeq & Ha'eq).
+    - pose(Hallows' := Hallows).
+      destruct Hallows' as (Hrinr & Hra & Hwb & Hwb').
+      assert (a <> a^+ 1)%a as Ha_a' by admit.
+      iMod "HRestrictRes" as (w1 w2) "(Ha & Ha' & HRestrictRes & #Hinterp_w1 & #Hinterp_w2)".
+      iExists _.
+      iSplitL "HRestrictRes".
+      + iSplitR; first auto.
+        case_decide as Hdec.
+        iExists w1, w2. iSplitR; auto.
+        exfalso; apply Hdec; auto.
+      + iModIntro; iNext. iFrame.
+        erewrite memMap_resource_2ne; auto ; iFrame.
+  Admitted.
+
+  Definition allow_read_IE_map_or_true (mem : Mem) (regs : Reg) (r : RegName) :=
+    ∃ p b e a,
+      read_reg_inr regs r p b e a ∧
+        if decide (reg_allows_read_IE regs r p b e a) then
+          ∃ w1 w2, mem !! a = Some w1 /\ mem !! (a^+1)%a = Some w2
+        else True.
+
+  Lemma mem_map_implies_pure_conds:
+    ∀ (mem : Mem) (regs : leibnizO Reg)
+      (pc_a : Addr) (pc_w : Word)
+      (dst : RegName) (p : Perm) (b e a : Addr) (Pa Pa': D) (f : bool),
+        allow_read_IE_mem mem regs dst pc_a pc_w p b e a Pa Pa' f
+        -∗ ⌜mem !! pc_a = Some pc_w⌝
+          ∗ ⌜allow_read_IE_map_or_true mem regs dst⌝.
+  Proof.
+  Admitted.
+
+  Lemma allow_read_IE_mem_later:
+    ∀ (mem : Mem) (regs : Reg) (dst : RegName)
+      (pc_a : Addr) (pc_w : Word)
+      (p : Perm) (b e a : Addr) (Pa Pa':D),
+      allow_read_IE_mem mem regs dst pc_a pc_w p b e a Pa Pa' true
+      -∗ ▷ allow_read_IE_mem mem regs dst pc_a pc_w p b e a Pa Pa' false.
+  Proof.
+    iIntros (mem regs dst pc_a pc_w p b e a Pa Pa' ) "HRestrictMem".
+  Admitted.
+
+  Instance if_Persistent regs dst pc_a p b e a w1 w2 :
+    Persistent (if decide (reg_allows_read_IE regs dst p b e a ∧ a ≠ pc_a ∧ (a ^+ 1)%a ≠ pc_a) then
+                  interp w1 ∗ interp w2 else emp)%I.
+  Proof. intros. destruct (decide (reg_allows_read_IE regs dst p b e a ∧ a ≠ pc_a ∧ (a ^+ 1)%a ≠ pc_a));apply _. Qed.
 
 
-  Lemma restrict_case (r : leibnizO Reg) (p : Perm)
-        (b e a : Addr) (widc w : Word) (dst : RegName) (r0 : Z + RegName) (P:D):
-    ftlr_instr r p b e a widc w (Restrict dst r0) P.
+   Lemma mem_map_recover_res:
+    ∀ (mem : Mem) (regs : leibnizO Reg)
+      (pc_a : Addr) (pc_w : Word) (dst : RegName)
+      (p : Perm) (b e a : Addr) (w1 w2 : Word) (Pa Pa' : D),
+      mem !! a = Some w1
+      -> mem !! (a ^+1)%a = Some w2
+      -> reg_allows_read_IE regs dst p b e a
+      → allow_read_IE_mem mem regs dst pc_a pc_w p b e a Pa Pa' false
+        -∗ ([∗ map] a'↦w' ∈ mem, a' ↦ₐ w')
+        ={(if decide (reg_allows_read_IE regs dst p b e a ∧ a ≠ pc_a ∧ (a ^+ 1)%a ≠ pc_a)
+          then ⊤ ∖ ↑logN.@pc_a ∖ ↑logN.@a ∖ ↑logN.@(a ^+ 1)%a
+          else ⊤ ∖ ↑logN.@pc_a),⊤ ∖ ↑logN.@pc_a}=∗
+          a ↦ₐ w1 ∗ (a ^+ 1)%a ↦ₐ w2 ∗
+          if decide (reg_allows_read_IE regs dst p b e a ∧ a ≠ pc_a ∧ (a ^+ 1)%a ≠ pc_a)
+          then interp w1 ∗ interp w2
+          else emp.
+  Proof.
+  Admitted.
+
+  Lemma read_IE_inr_eq {regs dst p b e a p' b' e' a'}:
+    reg_allows_read_IE regs dst p b e a →
+    read_reg_inr regs dst p' b' e' a' →
+    p = p' ∧ b = b' ∧ e = e' ∧ a = a'.
+  Proof.
+    intros Hrar Hrinr.
+    pose (Hrar' := Hrar).
+    destruct Hrar' as (Hinr0 & _). rewrite /read_reg_inr Hinr0 in Hrinr. by inversion Hrinr.
+  Qed.
+
+  Lemma restrict_case (regs : leibnizO Reg) (p_pc : Perm)
+        (b_pc e_pc a_pc : Addr) (widc wpc : Word) (dst : RegName) (r : Z + RegName) (P:D):
+    ftlr_instr regs p_pc b_pc e_pc a_pc widc wpc (Restrict dst r) P.
   Proof.
     intros Hp Hsome i Hbae Hi.
-    iIntros "#IH #Hinv_pc #Hinv_idc #Hinva #Hreg #[Hread Hwrite] Hown Ha HP Hcls HPC HIDC Hmap".
+    iIntros "#IH #Hinv_pc #Hinv_idc #Hinva #Hreg #[Hread Hwrite] Hown Hpc_a HP Hcls HPC HIDC Hmap".
     iInsertList "Hmap" [idc;PC].
 
+    (* To read out PC's name later, and needed when calling wp_restrict *)
+    assert(∀ x : RegName, is_Some (<[PC:=WCap p_pc b_pc e_pc a_pc]> regs !! x)) as Hsome'.
+    {
+      intros. destruct (decide (x = PC)) as [Heq|Heq].
+      rewrite Heq lookup_insert; unfold is_Some. by eexists.
+      by rewrite lookup_insert_ne.
+    }
 
-    (* TODO we need to do some manipulation in the resources here *)
+    assert (∃ p b e a, read_reg_inr (<[PC:=WCap p_pc b_pc e_pc a_pc]> regs) dst p b e a)
+      as (p & b & e & a & HVdst).
+    {
+      specialize Hsome' with dst as Hdst.
+      destruct Hdst as [wdst Hsomedst].
+      unfold read_reg_inr. rewrite Hsomedst.
+      destruct wdst as [|[ p b e a|] | ]; try done.
+      by repeat eexists.
+    }
 
-    iApply (wp_Restrict with "[$Ha $Hmap]"); eauto.
-    { simplify_map_eq; auto. }
+
+    destruct (decide (reg_allows_read_IE regs dst p b e a)) as [Hallows | Hallows].
+
+    - (* we can restrict to IE *)
+    - (* we can't restrict to IE -> the proof will be trivial *)
+
+
+    (* Step 1: open the region, if necessary,
+       and store all the resources obtained from the region
+       in allow_restrict_res *)
+    iDestruct (create_restrict_res with "Hreg") as (Pa Pa') "HRestrictRes"; eauto.
+    (* NOTE "HRestrictRes" describes the resources that we _can_ obtain:
+       - if the restricted capability can read `a` and `a+1`, then we can open the
+       invariant (which open the masks) and we can derive the points-to predicate.
+       - the restricted capability cannot read `a` and `a+1`, then we don't need to
+       open the invariant, because proving the LR for IE is trivial *)
+
+    (* Step2: derive the concrete map of memory we need,
+       and any spatial predicates holding over it *)
+    iMod (restrict_res_implies_mem_map with "HRestrictRes Hpc_a")
+      as (mem) "[HRestrictMem >[Hmem Hpc_a]]".
+    (* NOTE "HRestrictRes" describes the resources that we actually _own_.
+       It is a conditional over the reg_allows_read_IE, describes whether we
+       opened the invariant or not. *)
+
+    (* Step 3:  derive the non-spatial conditions over the memory map*)
+    iDestruct (mem_map_implies_pure_conds with "HRestrictMem") as %(HReadPC & HLoadAP); auto.
+
+    (* Step 4: move the later outside, so that we can remove it after applying wp_restrict *)
+    iDestruct (allow_read_IE_mem_later with "HRestrictMem") as "HRestrictMem"; auto.
+
+    iApply (wp_Restrict with "[$Hpc_a $Hmap]"); eauto.
+    { by simplify_map_eq. }
     { rewrite /subseteq /map_subseteq /set_subseteq_instance. intros rr _.
       apply elem_of_dom. apply lookup_insert_is_Some'; eauto.
       right. destruct (decide (rr = idc)); subst; simplify_map_eq; auto.
     }
 
-    iIntros "!>" (regs' retv). iDestruct 1 as (HSpec) "[Ha Hmap]".
+    (* Infer that if P holds at w, then w must be valid (read condition) *)
+    iDestruct ("Hread" with "HP") as "#Hw".
+
+    iIntros "!>" (regs' retv). iDestruct 1 as (HSpec) "[Hpc_a Hmap]".
     destruct HSpec as [ * Hdst HnE HnIE Hz Hfl HincrPC | * Hdst Hz Hfl HincrPC | ].
     { apply incrementPC_Some_inv in HincrPC as (p''&b''&e''&a''& ? & HPC & Z & Hregs') .
 
-      assert (a'' = a ∧ b'' = b ∧ e'' = e) as (-> & -> & ->).
+      assert (a'' = a_pc ∧ b'' = b_pc ∧ e'' = e_pc) as (-> & -> & ->).
       { destruct (decide (PC = dst)) ; simplify_map_eq; auto. }
 
       iApply wp_pure_step_later; auto.
-      iMod ("Hcls" with "[HP Ha]");[iExists w;iFrame|iModIntro].
-      iNext; iIntros "_".
 
-      (* TODO rewrite regs' to match with the induction hypothesis *)
-      iApply ("IH" $! regs' with "[%] [] [Hmap] [$Hown]").
-      { cbn. intros. subst regs'. by repeat (apply lookup_insert_is_Some'; right). }
-      { iIntros (ri v Hri Hri' Hvs).
-        subst regs'.
-        rewrite lookup_insert_ne in Hvs; auto.
-        destruct (decide (ri = dst)).
-        { simplify_map_eq.
-          unshelve iSpecialize ("Hreg" $! dst _ _ _ Hdst); eauto.
-          destruct (decide ((decodePerm n) = IE)) as [ Heq | Hneq]; simplify_eq ; cycle 1.
-           { iApply (interp_weakening with "IH Hreg") ; auto; solve_addr. }
-           rewrite Heq; rewrite Heq in Hfl; clear Heq.
-           admit. (* TODO lemma in case of IE *)
+      rewrite /allow_read_IE_map_or_true in HLoadAP.
+      destruct HLoadAP as (p' & b'& e'& a'& Hread & Hmem).
+
+      destruct (decide (reg_allows_read_IE (<[PC:=WCap p_pc b_pc e_pc a_pc]> regs) dst p b e a))
+      as [Hdec|Hdec].
+      +
+        (* destruct Hdec as (Hallows & Haeq & Ha'eq). *)
+        eapply read_IE_inr_eq in Hread; eauto.
+        destruct Hread as (<- & <- & <- & <-).
+        case_decide as Hcontra ; [|contradiction]; clear Hcontra.
+        destruct Hmem as (w1 & w2 & Hw1 & Hw2).
+
+        iMod (mem_map_recover_res with "HRestrictMem Hmem") as "(Ha & Ha' & #Hinterp)"
+        ;[eauto|eauto|auto|iModIntro].
+        (* destruct Hallows as (Hrinr & Hra & Hwb & Hwb'). *)
+
+        iMod ("Hcls" with "[HP Hpc_a]");[iExists wpc;iFrame|iModIntro].
+        (* Exceptional success case: we do not apply the induction hypothesis in case
+           we have a faulty PC *)
+        destruct (decide (p'' = RX ∨ p'' = RWX)).
+        2 : {
+          assert (p'' ≠ RX ∧ p'' ≠ RWX). split; by auto.
+          iDestruct ((big_sepM_delete _ _ PC) with "Hmap") as "[HPC Hmap]".
+          { subst. by rewrite lookup_insert. }
+          iNext; iIntros "_".
+          iApply (wp_bind (fill [SeqCtx])).
+          iApply (wp_notCorrectPC_perm with "[HPC]"); eauto. iIntros "!> _".
+          iApply wp_pure_step_later; auto.
+          iNext; iIntros "_".
+          iApply wp_value.
+          iIntros (a1); inversion a1.
+        }
+
+
+        iAssert (
+            ∀ (r0 : RegName) (v : leibnizO Word),
+              ⌜r0 ≠ PC⌝ → ⌜r0 ≠ idc⌝ → ⌜regs' !! r0 = Some v⌝ → fixpoint interp1 v
+          )%I with "[Hmap Ha Ha']" as "Hinterp_reg".
+        { iIntros (ri v Hri Hri' Hvs).
+          subst regs'.
+          rewrite lookup_insert_ne in Hvs; auto.
+          destruct (decide (ri = dst)).
+          { simplify_map_eq.
+            unshelve iSpecialize ("Hreg" $! dst _ _ _ Hdst); eauto.
+            destruct (decide ((decodePerm n) = IE)) as [ Heq | Hneq]; simplify_eq ; cycle 1.
+            { iApply (interp_weakening with "IH Hreg") ; auto; solve_addr. }
+            rewrite Heq; rewrite Heq in Hfl; clear Heq.
+            simplify_map_eq.
+
+            admit. (* TODO lemma in case of IE *)
+
+          }
+          { repeat (rewrite lookup_insert_ne in Hvs); auto.
+            iApply "Hreg"; auto. } }
 
         }
-        { repeat (rewrite lookup_insert_ne in Hvs); auto.
-          iApply "Hreg"; auto. } }
+
+        iNext; iIntros "_".
+        (* TODO rewrite regs' to match with the induction hypothesis *)
+        iApply ("IH" $! regs' with "[%] [] [Hmap] [$Hown]").
+        { cbn. intros. subst regs'. by repeat (apply lookup_insert_is_Some'; right). }
+        { iIntros (ri v Hri Hri' Hvs).
+          subst regs'.
+          rewrite lookup_insert_ne in Hvs; auto.
+          destruct (decide (ri = dst)).
+          { simplify_map_eq.
+            unshelve iSpecialize ("Hreg" $! dst _ _ _ Hdst); eauto.
+            destruct (decide ((decodePerm n) = IE)) as [ Heq | Hneq]; simplify_eq ; cycle 1.
+            { iApply (interp_weakening with "IH Hreg") ; auto; solve_addr. }
+            rewrite Heq; rewrite Heq in Hfl; clear Heq.
+            rewrite /allow_restrict_res.
+            admit. (* TODO lemma in case of IE *)
+
+          }
+          { repeat (rewrite lookup_insert_ne in Hvs); auto.
+            iApply "Hreg"; auto. } }
         { subst regs'. rewrite insert_insert. iApply "Hmap". }
-      iModIntro.
-      iApply (interp_weakening with "IH Hinv"); auto; try solve_addr.
-      { destruct Hp; by subst p. }
-      { destruct (reg_eq_dec PC dst) as [Heq | Hne]; simplify_map_eq.
-        auto. by rewrite PermFlowsToReflexive. }
+        iModIntro.
+        iApply (interp_weakening with "IH Hinv"); auto; try solve_addr.
+        { destruct Hp; by subst p. }
+        { destruct (reg_eq_dec PC dst) as [Heq | Hne]; simplify_map_eq.
+          auto. by rewrite PermFlowsToReflexive. }
     }
     { apply incrementPC_Some_inv in HincrPC as (p''&b''&e''&a''& ? & HPC & Z & Hregs') .
 
@@ -203,7 +431,7 @@ Section fundamental.
       { destruct Hp; by subst p. }
       { by rewrite PermFlowsToReflexive. }
     }
-     { iApply wp_pure_step_later; auto.
+    { iApply wp_pure_step_later; auto.
       iMod ("Hcls" with "[HP Ha]");[iExists w;iFrame|iModIntro].
       iNext; iIntros "_".
       iApply wp_value; auto. iIntros; discriminate. }
